cfrontend/Csyntax.v
@@ -64,10 +64,12 @@ Inductive expr : Type :=
 | Ecall (r1: expr) (rargs: exprlist) (ty: type)             (**r function call [r1(rargs)] *)
 | Ebuiltin (ef: external_function) (tyargs: typelist) (rargs: exprlist) (ty: type)
                                                                 (**r builtin function call *)
-| Eloc (ofs: ptrofs) (pt:tag) (bf: bitfield) (ty: type)
+| Eloc (ofs: ptrofs) (pt: tag) (bf: bitfield) (ty: type)
                                       (**r memory location, result of evaluating a l-value *)
+| Efloc (b: block) (pt: tag) (ty: type)          (**r function "location," also an l-value *)
 | Eparen (r: expr) (tycast: type) (ty: type)                     (**r marked subexpression *)
-
+| Efailstop (ty: type)
+         
 with exprlist : Type :=
   | Enil
   | Econs (r1: expr) (rl: exprlist).
@@ -126,6 +128,7 @@ Definition Eselection (r1 r2 r3: expr) (ty: type) :=
 Definition typeof (a: expr) : type :=
   match a with
   | Eloc _ _ _ ty => ty
+  | Efloc _ _ ty => ty
   | Evar _ ty => ty
   | Ederef _ ty => ty
   | Efield _ _ ty => ty
@@ -147,6 +150,7 @@ Definition typeof (a: expr) : type :=
   | Ecall _ _ ty => ty
   | Ebuiltin _ _ _ ty => ty
   | Eparen _ _ ty => ty
+  | Efailstop ty => ty
   end.
 
 (** ** Statements *)
